src/impl/TLS13.Impl.Client.Driver.Cleanup.fsti
@@ -5,6 +5,7 @@ module TLS13.Impl.Client.Driver.Cleanup
 open Pulse.Lib.Pervasives
 
 module B = TLS13.Bytes
+module BT = Common.BufferedTCP
 module C = TLS13.Impl.Client
 module DS = TLS13.Impl.Client.Driver.State
 module IO = Common.TCP
@@ -16,32 +17,31 @@ module SZ = FStar.SizeT
 inline_for_extraction
 fn free_client_driver_buffers
   (d:DS.client_driver)
-  (buffered_len:SZ.t)
-  requires (exists* buffered. DS.client_driver_buffers d buffered buffered_len)
+  requires DS.client_driver_buffers d
   ensures emp
 
 inline_for_extraction
 fn free_disconnected_client_driver
   (d:DS.client_driver)
-  (buffered_len:SZ.t)
   requires C.connection_exactly d.DS.client_driver_client 'st0 **
            DS.client_driver_canonical_progress d 'st0 **
            O.is_auth_context d.DS.client_driver_auth **
            Box.pts_to d.DS.client_driver_channel DS.no_channel **
            (exists* h. MR.pts_to d.DS.client_driver_tcp_history #1.0R h) **
-           (exists* buffered.
-             DS.client_driver_buffers d buffered buffered_len)
+           DS.client_driver_buffers d **
+           (exists* model.
+             BT.is_storage d.DS.client_driver_storage model)
   ensures DS.client_driver_closed d 'st0
 
 inline_for_extraction
 fn close_failed_connect
   (d:DS.client_driver)
-  (ch:IO.channel)
-  (buffered_len:SZ.t)
-  requires C.connection_exactly d.DS.client_driver_client 'st0 **
-           DS.client_driver_canonical_progress d 'st0 **
-           O.is_auth_context d.DS.client_driver_auth **
-           DS.channel_open d.DS.client_driver_tcp_history ch 'st0 'buffered buffered_len **
+  (channel:BT.t)
+  requires DS.top_buffered_driver_exactly
+             (DS.client_top_buffered_driver d channel)
+             'st0
+             'buffered
+             'buffered_len **
            Box.pts_to d.DS.client_driver_channel DS.no_channel **
-           DS.client_driver_buffers d (Ghost.reveal 'buffered) buffered_len
+           DS.client_driver_buffers d
   ensures DS.client_driver_closed d 'st0
